src/IsoCan.v
@@ -4,6 +4,7 @@ Unset Strict Implicit.
 Unset Printing Implicit Defensive.
 From RDF Require Export Rdf Triple Term Util.
 
+
 Section HashedData.
 
   (* A type for a data (t : T) paired with its current hash (h : H) *)
@@ -668,20 +669,16 @@ Section IsoCan.
           else
             b.
 
-      (* Definition k_mapping_ts (ts : seq (triple I B L)) : seq (triple I B L) := *)
-      (*   let all_maps := *)
-      (*     map (mapi (app_n mark_bnode)) (permutations (bnodes_ts (init_hash_ts ts))) in *)
-      (*   let mus := map build_kmapping_from_seq all_maps in *)
-      (*   let isocans := map (fun mu => (relabeling_seq_triple mu ts)) mus in *)
-      (*   foldl Order.max [::] isocans. *)
-      (* The term "[::]" has type "seq ?T0" while it is expected to have type "Order.POrder.sort ?T". *)
+
+      Definition k_mapping_ts (ts : seq (triple I B L)) : seq (triple I B L) :=
+        let all_maps :=
+          map (mapi (app_n mark_bnode)) (permutations (bnodes_ts (init_hash_ts ts))) in
+        let mus := map build_kmapping_from_seq all_maps in
+        let isocans := map (fun mu => (relabeling_seq_triple mu ts)) mus in
+        foldl Order.max [::] isocans.
 
       Definition k_mapping (g : rdf_graph I B L) : rdf_graph I B L :=
-        let all_maps :=
-          map (mapi (app_n mark_bnode)) (permutations (bnodes (init_hash g))) in
-        let mus := map build_kmapping_from_seq all_maps in
-        let isocans := map (fun mu => (@relabeling _ _ _ _ mu g todo)) mus in
-        foldl Order.max empty_rdf_graph isocans.
+        @mkRdfGraph I B L (k_mapping_ts (graph g)) todo.
 
       Lemma k_mapping_seq_uniq_ts ts: uniq (mapi (app_n mark_bnode) (bnodes_ts (init_hash_ts ts))).
       Proof.
